theories/iris_fundamental.v
@@ -74,38 +74,6 @@ Section fundamental.
   Proof.
     induction vs;auto. Qed.
 
-
-
-
-  (* --------------------------------------------------------------------------------------- *)
-  (* -------------------------------------- EXPRESSIONS ------------------------------------ *)
-  (* --------------------------------------------------------------------------------------- *)
-
-  Lemma typing_const C v : ⊢ semantic_typing (HWP:=HWP) C (to_e_list [BI_const v]) (Tf [] [typeof v]).
-  Proof.
-    unfold semantic_typing, interp_expression.
-    iIntros (i lh f vs).
-    iIntros "#Hi [%Hlh_base [%Hlh_len #Hcont]] #Hv".
-    iExists (LH_base [] []). iSplit;auto.
-    iIntros "Hf".
-    iApply wp_wasm_empty_ctx.
-    iDestruct "Hf" as (locs Heq) "[#Hlocs Hf]".
-    iDestruct "Hv" as "[-> | Hv]".
-    { take_drop_app_rewrite_twice 0 1.
-      iApply (wp_wand_r _ _ _ (λ vs, interp_val [typeof v] vs ∗  ↪[frame]f)%I). iSplitL.
-      { iApply (wp_trap with "[] [$]");auto. by iLeft. }
-      iIntros (v0) "[? ?]". iFrame. iExists _. iFrame. }
-    { iDestruct "Hv" as (ws ->) "Hv".
-      iDestruct (big_sepL2_nil_inv_r with "Hv") as %->.
-      iApply (wp_wand_r _ _ _ (λ vs, interp_val [typeof v] vs ∗  ↪[frame]f)%I). iSplitL.
-      { rewrite app_nil_l.
-        iApply wp_value;[by instantiate (1:= immV [_])|].
-        iFrame. iRight. iExists _. iSplit;eauto.
-        iSimpl; iSplit =>//. iApply interp_value_type_of. }
-      iIntros (v0) "[? ?]". iFrame. iExists _. iFrame. 
-    }
-  Qed.
-
   Lemma lh_depth_push_base lh n es es1 vs2 :
     lh_depth (push_base lh n es es1 vs2) = S (lh_depth lh).
   Proof.
@@ -122,18 +90,300 @@ Section fundamental.
       simpl. auto. }
   Qed.
 
-  Lemma interp_ctx_push_label C tm i lh tn ws es :
+  Lemma lh_minus_base_is_empty lh l1 l2 :
+    is_Some (lh_minus lh (LH_base l1 l2)) -> l1 = [] ∧ l2 = [].
+  Proof.
+    intros [lh' Hsome].
+    apply lh_minus_Ind_Equivalent in Hsome.
+    inversion Hsome;subst;auto.
+  Qed.
+
+  Lemma lh_minus_push_base_is_Some lh n es es1 es2 lh'' :
+    lh_depth lh'' <= lh_depth lh ->
+    is_Some (lh_minus (push_base lh n es es1 es2) lh'') ->
+    is_Some (lh_minus lh lh'').
+  Proof.
+    revert lh'' n es es1 es2. induction lh;intros lh'' m es es1 es2 Hlt Hsome.
+    { simpl in Hlt. destruct lh'';simpl in *.
+      { destruct l1;[|done].
+        destruct l2;[|done].
+        eauto. }
+      { lia. }
+    }
+    { simpl in Hlt.
+      destruct lh''.
+      { destruct l2,l3; done. }
+      { simpl in Hsome. simpl.
+        destruct ((l == l2) && (n =? n0) && (l0 == l3) && (l1 == l4));[|done].
+        simpl in Hlt. apply le_S_n in Hlt.
+        eapply IHlh in Hlt;eauto.
+      }
+    }
+  Qed.
+
+  Lemma get_layer_push_base_0 lh n es vs1 es1 :
+    base_is_empty lh ->
+    get_layer (push_base lh n es vs1 es1) (lh_depth lh) = Some ([],n,es,LH_base vs1 es1,[]).
+  Proof.
+    induction lh;intros Hemp.
+    { simpl in *. destruct Hemp as [-> ->]. eauto. }
+    { simpl in *. eauto. }
+  Qed.
+
+  Lemma lh_depth_eq_lh_minus lh'' lh n es vs1 es1 :
+    base_is_empty lh ->
+    lh_depth lh'' = lh_depth lh ->
+    is_Some (lh_minus (push_base lh n es vs1 es1) lh'') ->
+    lh'' = lh.
+  Proof.
+    revert lh n es vs1 es1.
+    induction lh'';intros lh m es vs1 es1 Hbase Hdep [lh' Hsome].
+    { destruct lh;[|done]. simpl in *.
+      destruct l,l0;try done.
+      destruct Hbase as [-> ->];auto. }
+    { destruct lh;[done|]. simpl in *.
+      inversion Hdep as [Hdep'].
+      destruct ((l2 == l) && (n0 =? n) && (l3 == l0) && (l4 == l1)) eqn:Heq;[|done].
+      eapply IHlh'' in Hdep' as ->;eauto.
+      revert Heq. rewrite !andb_true_iff =>Heq.
+      destruct Heq as [[[->%ai_eqseq_true ->%PeanoNat.Nat.eqb_eq] ->%ai_eqseq_true] ->%ai_eqseq_true].
+      auto. }
+  Qed.
+
+  Lemma lholed_lengths_gt0_get_snoc lh lbs :
+    lh_depth lh > 0 ->
+    lholed_lengths (rev lbs) lh ->
+    ∃ lbs' tc, lbs = lbs' ++ [tc].
+  Proof.
+    induction lbs using rev_ind;intros Hlh Hh.
+    { destruct lh;[simpl in Hlh;lia|done]. }
+    { eauto. }
+  Qed.
+
+  Lemma of_val_length ws :
+    length (of_val (immV ws)) = length ws.
+  Proof.
+    by rewrite fmap_length.
+  Qed.
+
+  Lemma base_is_empty_push_base lh n es :
+    base_is_empty (push_base lh n es [] []).
+  Proof.
+    induction lh;simpl;auto.
+  Qed.
+
+  Lemma lholed_lengths_push_base lh l tn es :
+    lholed_lengths l lh ->
+    lholed_lengths (l ++ [tn]) (push_base lh (length tn) es [] []).
+  Proof.
+    revert lh. induction l;intros lh Hlh.
+    { destruct lh;inversion Hlh. simpl. eauto. }
+    { destruct lh;inversion Hlh. simpl. split;auto. }
+  Qed.
+
+  Lemma lholed_valid_push_base lh n es :
+    lholed_valid lh ->
+    lholed_valid (push_base lh n es [] []).
+  Proof.
+    intros Hlh;induction lh.
+    { simpl in *. auto. }
+    { inversion Hlh. simpl. split;auto. }
+  Qed.
+
+  Lemma lfilledInd_push_inv i : ∀ lh n es' es LI l1 l2,
+      const_list l1 ->
+      lfilledInd (S i) (push_base lh n es' l1 l2) es LI ->
+      lfilledInd i lh ([::AI_label n es' (l1 ++ es ++ l2)]) LI.
+  Proof.
+    induction i.
+    all: intros lh n es' es LI l1 l2 Hconst Hfill.
+    { inversion Hfill;subst.
+      destruct lh.
+      { simpl in H0. simplify_eq.
+        inversion H2. constructor. auto. }
+      { simpl in H0. simplify_eq. destruct lh;inversion H2. }
+    }
+    { inversion Hfill;subst. simpl.
+      destruct lh.
+      { simpl in H0. simplify_eq.
+        inversion H2. }
+      { simpl in H0. simplify_eq.
+        constructor; auto. 
+      }
+    }
+  Qed.
+
+  Lemma wp_label_push_inv (s : stuckness) (E : coPset) (Φ : val -> iProp Σ) es i lh n es' l1 l2 :
+    const_list l1 ->
+    WP [::AI_label n es' (l1 ++ es ++ l2)] @ s; E CTX i; lh {{ Φ }}
+    ⊢ WP es @ s; E CTX S i; push_base lh n es' l1 l2 {{ Φ }}.
+  Proof.
+    iIntros (Hconst) "HWP".
+    iIntros (LI Hfill%lfilled_Ind_Equivalent).
+    apply lfilledInd_push_inv in Hfill;auto.
+    iDestruct ("HWP" with "[]") as "HWP";[|iFrame].
+    iPureIntro. by apply lfilled_Ind_Equivalent.
+  Qed.
+  Lemma wp_label_push_nil_inv (s : stuckness) (E : coPset) (Φ : val -> iProp Σ) es i lh n es' :
+    WP [::AI_label n es' es] @ s; E CTX i; lh {{ Φ }}
+    ⊢ WP es @ s; E CTX S i; push_base lh n es' [] [] {{ Φ }}.
+  Proof.
+    iIntros "HWP".
+    iDestruct (wp_label_push_inv with "[HWP]") as "HWP";auto.
+    { auto. }
+    erewrite app_nil_l. erewrite app_nil_r. done.
+  Qed.
+
+  Lemma push_base_return v lh tm n es f :
+    lholed_valid lh ->
+    interp_val tm (immV v) -∗
+    ↪[frame] f -∗
+    (↪[frame] f -∗ WP of_val (immV v) CTX lh_depth lh; lh {{ vs, interp_val tm vs ∗ ∃ f, ↪[frame]f }}) -∗
+    WP of_val (immV v) CTX S (lh_depth lh); push_base lh n es [] []
+                    {{ vs, interp_val tm vs ∗ ∃ f, ↪[frame]f }}.
+  Proof.
+    iInduction lh as [] "IH".
+    { simpl. iIntros (Hvalid) "#Hv Hf H".
+      iApply (wp_val_return' with "[$Hf] [H]").
+      { apply const_list_of_val. }
+      { iIntros "Hf". iApply wp_wasm_empty_ctx.
+        iApply wp_base_push;auto. simpl. erewrite app_nil_r.
+        iApply "H". iFrame.
+      }
+    }
+    { iIntros (Hvalid) "#Hv Hf H".
+      iApply (wp_label_push_nil_inv with "[Hf H]").
+      iSimpl.
+      iApply iRewrite_nil_r_ctx.
+      iApply (wp_seq_can_trap_ctx _ _ _
+                (λ vs, (⌜vs = immV v⌝ ∗ ([∗ list] w;τ ∈ v;tm, interp_value τ w))))%I.
+      iFrame.
+      iSplitR.
+      { iIntros "Hcontr".
+        iDestruct "Hcontr" as "[%Hcontr _]". done. }
+      iSplitR;[auto|].
+      iSplitR.
+      { iIntros "Hf".
+        iApply (wp_wand _ _ _ (λ w, (⌜w = trapV⌝ ∨ ⌜w = immV v⌝ ∗ ([∗ list] w0;τ ∈ v;tm, interp_value τ w0)) ∗ ↪[frame] f)%I with "[Hf]").
+        { iApply (wp_label_value with "Hf");[by rewrite of_val_imm to_of_val|].
+          iDestruct "Hv" as "[%Hcontr | #Hv]";[done|].
+          iDestruct "Hv" as (ws Heq) "Hv". simplify_eq.
+          auto. }
+        { iIntros (v0) "[Hv0 Hf]".
+          iSplitR "Hf";[|eauto]. auto. } }
+      { iIntros (w) "[[-> Hw] Hf0]".
+        rewrite app_nil_r. iApply "H". iFrame.
+      }
+    }
+  Qed.
+
+  (* --------------------------------------------------------------------------------------- *)
+  (* -------------------------------------- EXPRESSIONS ------------------------------------ *)
+  (* --------------------------------------------------------------------------------------- *)
+
+  
+  (* ----------------------------------------- CONST --------------------------------------- *)
+  
+  Lemma typing_const C v : ⊢ semantic_typing (HWP:=HWP) C (to_e_list [BI_const v]) (Tf [] [typeof v]).
+  Proof.
+    unfold semantic_typing, interp_expression.
+    iIntros (i lh).
+    iIntros "#Hi [%Hlh_base [%Hlh_len [%Hlh_valid #Hcont]]]".
+    iIntros (f vs) "Hf #Hv".
+    iDestruct "Hf" as (locs Heq) "[#Hlocs Hf]".
+    iDestruct "Hv" as "[-> | Hv]".
+    { take_drop_app_rewrite_twice 0 1.
+      iApply (wp_wand_ctx _ _ _ (λ vs, ⌜vs = trapV⌝ ∗  ↪[frame]f)%I with "[Hf]").
+      { iApply (wp_trap_ctx with "[$]");auto. }
+      iIntros (v0) "[? ?]". iFrame. iExists _. iFrame. }
+    { iDestruct "Hv" as (ws ->) "Hv".
+      iDestruct (big_sepL2_nil_inv_r with "Hv") as %->.
+      iDestruct "Hcont" as "[_ Hcont]".
+      rewrite app_nil_l. iSimpl.
+      unfold interp_ctx_return, interp_expression.
+      assert ([AI_basic (BI_const v)] = of_val (immV [v])) as ->;auto.
+      iApply "Hcont".
+      { iRight. iExists _. iSplit;eauto.
+        iSimpl; iSplit =>//. iApply interp_value_type_of. }
+      iExists _. iFrame. eauto. }
+  Qed.
+
+  (* ----------------------------------------- LOOP ---------------------------------------- *)
+   
+  Lemma interp_ctx_continuations_push_label_loop lh C i tm tn es :
+    base_is_empty lh ->
+    lholed_lengths (rev (tc_label C)) lh ->
+    □ (∀ (a : leibnizO frame) (a0 : seq.seq value),
+           ⌜a = {| f_locs := a0; f_inst := i |}⌝
+           → ∀ a1 : seq.seq (leibnizO value),
+               ⌜length a1 = length tn⌝
+               →  ↪[frame]a -∗
+                 □ interp_val (tc_local C) (immV a0) -∗
+                 □ ([∗ list] w;τ ∈ a1;tn, interp_value τ w) -∗
+                 WP of_val (immV a1) ++ to_e_list [BI_loop (Tf tn tm) es]
+                 CTX
+                 lh_depth lh; lh
+                 {{ vs, interp_val tm vs ∗
+                    (∃ f0 : leibnizO frame,  ↪[frame]f0) }}) -∗
+    interp_ctx_continuations (tc_label C) tm (tc_local C) i lh -∗
+    interp_ctx_continuations [tn]
+                             tm
+                             (tc_local (upd_label C ([tn] ++ tc_label C)%list))
+                             i
+                             (push_base lh (length tn) [AI_basic (BI_loop (Tf tn tm) es)] [] []).
+  Proof.
+    iIntros (Hlh_base Hlh_len) "#HIH #Hc".
+    iSimpl. rewrite lh_depth_push_base.
+    assert (S (lh_depth lh) - 1 = lh_depth lh) as ->;[lia|].
+    rewrite get_layer_push_base_0;[|auto].
+    iSplit;[|done].
+    iExists _,_,_,_,_. iSplit;[eauto|].
+    iModIntro. iIntros (v f lh'' [Hdep Hmin]).
+    iIntros "#Hw Hf".
+    iDestruct "Hf" as (locs Heqf) "[#Hlocs Hf]".
+    apply lh_depth_eq_lh_minus in Hmin as Heq;auto.
+    subst lh''.
+    unfold interp_expression.
+    rewrite app_nil_l app_nil_r.
+
+    iDestruct "Hw" as "[-> | Hv]".
+    { iClear "HIH".
+      take_drop_app_rewrite_twice 0 1.
+      iApply (wp_wand_ctx _ _ _ (λ vs, ⌜vs = trapV⌝ ∗  ↪[frame]f)%I with "[Hf]").
+      { iApply (wp_trap_ctx with "[Hf]");auto. }
+      iIntros (v0) "[? ?]". iFrame. iExists _. iFrame. }
+
+    iDestruct "Hv" as (ws' ->) "Hv".
+    iDestruct (big_sepL2_length with "Hv") as %Hlen.
+    
+    iDestruct ("HIH" with "[] [] [Hf] [] []") as "Hcont";eauto.
+  Qed.
+
+  Lemma interp_ctx_push_label_loop C tm i lh tn es :
+    □ (∀ (a : leibnizO frame) (a0 : seq.seq value),
+           ⌜a = {| f_locs := a0; f_inst := i |}⌝
+           → ∀ a1 : seq.seq (leibnizO value),
+               ⌜length a1 = length tn⌝
+               →  ↪[frame]a -∗
+                 □ interp_val (tc_local C) (immV a0) -∗
+                 □ ([∗ list] w;τ ∈ a1;tn, interp_value τ w) -∗
+                 WP of_val (immV a1) ++ to_e_list [BI_loop (Tf tn tm) es]
+                 CTX
+                 lh_depth lh; lh
+                 {{ vs, interp_val tm vs ∗
+                    (∃ f0 : leibnizO frame,  ↪[frame]f0) }}) -∗
     interp_ctx (tc_label C) tm (tc_local C) i lh -∗
     interp_ctx (tc_label (upd_label C ([tn] ++ tc_label C)%list)) tm
       (tc_local (upd_label C ([tn] ++ tc_label C)%list)) i
-      (push_base lh (length (of_val (immV ws))) [AI_basic (BI_loop (Tf tn tm) es)] [] []).
+      (push_base lh (length tn) [AI_basic (BI_loop (Tf tn tm) es)] [] []).
   Proof.
-    iIntros "[%Hlh_base [%Hlh_len #Hc]]".
-    iSplit;[|iSplit].
-    { admit. }
-    { admit. }
+    iIntros "#HIH [%Hlh_base [%Hlh_len [%Hlh_valid #[Hc Hr]]]]".
+    iSplit;[|iSplit;[|iSplit;[|iSplit]]].
+    { iPureIntro. apply base_is_empty_push_base. }
+    { iPureIntro. apply lholed_lengths_push_base. auto. }
+    { iPureIntro. apply lholed_valid_push_base. auto. }
     { iSplitR.
-      { admit. }
+      { iApply (interp_ctx_continuations_push_label_loop with "[] []");auto. }
       iApply (big_sepL_mono with "Hc").
       iIntros (k y Hk). iSimpl.
       iIntros "#Hcont".
@@ -144,87 +394,63 @@ Section fundamental.
       { iPureIntro. apply get_layer_push_base;eauto. }
       iModIntro. iIntros (v f lh'' [Hdep Hmin]) "#Hv Hf".
       iDestruct "Hf" as (locs Heq) "[#Hlocs Hf]".
-      rewrite PeanoNat.Nat.sub_succ in Hdep.
       iApply ("Hcont" with "[] Hv [Hf]").
-      { iPureIntro. split;auto. admit. }
+      { iPureIntro. split;auto. eapply lh_minus_push_base_is_Some;eauto. lia. }
       iExists _. iFrame. eauto.
     }
-  Admitted.
-
-      
+    { unfold interp_ctx_return. iModIntro. iIntros (v f) "#Hv Hf".
+      iDestruct ("Hr" $! _ f with "Hv") as "Hr'".
+      iDestruct "Hf" as (locs Heq) "[#Hlocs Hf]".
+      iDestruct "Hv" as "[-> | Hv]".
+      { unfold interp_expression. iSimpl. iClear "#".
+        take_drop_app_rewrite_twice 0 0.
+        iApply (wp_wand_ctx with "[Hf]").
+        { iApply wp_trap_ctx;eauto. }
+        iIntros (v) "[H Hf]". iSplitR "Hf";eauto. }
+      iDestruct "Hv" as (ws ->) "Hv".
+      unfold interp_expression. rewrite lh_depth_push_base.
+      iApply (push_base_return with "[] [Hf] []");auto.
+      { iRight. eauto. }
+      { iIntros "Hf". iApply "Hr'". iExists _. eauto. }
+    }
+  Qed.
     
   Lemma typing_loop C es tn tm : (⊢ semantic_typing (HWP:=HWP) (upd_label C ([tn] ++ tc_label C)%list) (to_e_list es) (Tf tn tm)) ->
                                  ⊢ semantic_typing (HWP:=HWP) C (to_e_list [BI_loop (Tf tn tm) es]) (Tf tn tm).
   Proof.
     intros IHbe_typing.
     unfold semantic_typing, interp_expression.
-    iIntros (i lh f vs).
-    iIntros "#Hi #Hc #Hv".
+    iIntros (i lh).
+    iIntros "#Hi".
+    
+    iDestruct (IHbe_typing $! i (push_base lh (length tn) [AI_basic (BI_loop (Tf tn tm) es)]
+                                           [] []) with "[]") as "HH"; [by (destruct C,i;eauto)|].
+
+    iIntros "#Hc". iIntros (f vs) "Hf #Hv".
+    iDestruct "Hf" as (locs Heq) "[#Hlocs Hf]".
     
     iDestruct "Hv" as "[-> | Hv]".
-    { iExists (LH_base [] []). iSplit;auto.
-      iIntros "Hf".
-      iApply wp_wasm_empty_ctx.
-      iDestruct "Hf" as (locs Heq) "[#Hlocs Hf]". 
-      take_drop_app_rewrite_twice 0 1.
-      iApply (wp_wand_r _ _ _ (λ vs, interp_val tm vs ∗  ↪[frame]f)%I). iSplitL.
-      { iApply (wp_trap with "[] [$]");auto. by iLeft. }
-      iIntros (v0) "[? ?]". iFrame. iExists _. iFrame. }
+    {  take_drop_app_rewrite_twice 0 1.
+       iApply (wp_wand_ctx _ _ _ (λ vs, ⌜vs = trapV⌝ ∗  ↪[frame]f)%I with "[Hf]").
+       { iApply (wp_trap_ctx with "[Hf]");auto. }
+       iIntros (v0) "[? ?]". iFrame. iExists _. iFrame. }
     iDestruct "Hv" as (ws ->) "Hv".
     iDestruct (big_sepL2_length with "Hv") as %Hlen.
-    
-    iDestruct (IHbe_typing with "[] [] []") as (lh') "[%Hlh' HH]";try by (destruct C,i;eauto).
-    { instantiate (1:=push_base lh (length (of_val (immV ws))) [AI_basic (BI_loop (Tf tn tm) es)] [] []).
-      iApply interp_ctx_push_label. iFrame "Hc".}
-    { instantiate (1:=immV ws). iRight. eauto. }
 
-    destruct Hlh' as [-> | ->].
-
-    { iExists lh. iSplit;auto.
-      iIntros "Hf".
-      iDestruct "Hf" as (locs Heq) "[#Hlocs Hf]".
-      iAssert (↪[frame]f -∗ WP of_val (immV ws) ++ to_e_list es CTX S (lh_depth lh);
-               push_base lh (length (of_val (immV ws))) [AI_basic (BI_loop (Tf tn tm) es)] [] []
-                {{ vs, interp_val tm vs ∗ (∃ f0 : leibnizO frame,  ↪[frame]f0) }})%I as "Hcontlh'".
-      { iIntros "Hf". unfold interp_expression. rewrite lh_depth_push_base. iApply ("HH"). iFrame. iExists _. eauto. }
-      iApply (wp_loop_ctx with "Hf");eauto.
-      { apply v_to_e_is_const_list. }
-      { rewrite fmap_length //. }
-      iNext. iIntros "Hf".
-      iApply wp_label_push_nil. iApply "Hcontlh'". iFrame. }
-
-    { iExists (LH_base [] []). iSplit;auto.
-      iIntros "Hf".
-      iDestruct "Hf" as (locs Heq) "[#Hlocs Hf]".
-      iAssert (↪[frame]f -∗ WP of_val (immV ws) ++ to_e_list es
-                {{ vs, interp_val tm vs ∗ (∃ f0 : leibnizO frame,  ↪[frame]f0) }})%I as "Hcontlh'".
-      { iIntros "Hf". unfold interp_expression. iApply wp_wasm_empty_ctx. iApply "HH". iFrame. iExists _. eauto. }
-      iSimpl.
-      iApply wp_wasm_empty_ctx.
-      iApply (wp_loop with "Hf");eauto.
-      { apply v_to_e_is_const_list. }
-      { rewrite fmap_length //. }
-      iNext. iIntros "Hf".
-      iApply wp_wasm_empty_ctx.
-      iApply wp_label_push_nil.
-      iApply iRewrite_nil_r_ctx.
-      iApply wp_seq_can_trap_ctx. iFrame "∗ #". 
-      iSplitR.
-      { iIntros "Hcontr". simpl.
-        iDestruct "Hcontr" as (ws0 Hcontr) "_". done. }
-      iSplitR.
-      { iLeft. auto. }
-      iIntros (w f0) "Hres".
-      iDestruct "Hres" as "[Hw Hf]".
-      iDestruct "Hw" as (vs ->) "Hvs".
-      rewrite app_nil_r. simpl push_base.
-      iApply (wp_wand_ctx with "[-]").
-      { iApply (wp_val_return with "Hf").
-        { apply const_list_of_val. }
-        iIntros "Hf". iFrame.
-        instantiate (1:=interp_val tm).
-        iApply wp_value;[by rewrite app_nil_l app_nil_r|iRight;eauto]. }
-      { iIntros (v) "[Hw Hf]". iFrame. eauto. } }
+    iRevert "Hlocs Hv". iLöb as "IH"
+  forall (f locs Heq ws Hlen).
+    iIntros "#Hlocs #Hv".
+    iApply (wp_loop_ctx with "Hf");eauto.
+    { apply v_to_e_is_const_list. }
+    { rewrite fmap_length //. }
+    iNext. iIntros "Hf".
+    iApply wp_label_push_nil.
+    iDestruct ("HH" with "[] [Hf] []") as "Hcont".
+    { iApply (interp_ctx_push_label_loop with "[$] [$]"). }
+    { iExists _. iFrame "∗ #". auto. }
+    { iFrame "#". iRight. iExists _. eauto. }
+    unfold interp_expression. rewrite lh_depth_push_base.
+    rewrite of_val_length Hlen. iFrame. 
   Qed.
     
   (* --------------------------------------------------------------------------------------- *)
